duals and loops

src/matroid/ncard/dual.lean
@@ -1,4 +1,4 @@
-import .flat
+import .loop
 
 noncomputable theory
 
@@ -9,20 +9,24 @@ variables {E : Type*} [finite E] {M M₁ M₂ : matroid E} {B B₁ B₂ X Y Z : 
 open set
 namespace matroid 
 
-lemma base.strong_exchange (hB₁ : M.base B₁) (hB₂ : M.base B₂) (hx : x ∈ B₁ \ B₂) :
-  ∃ y ∈ B₂ \ B₁, M.base (insert x (B₂ \ {y})) ∧ M.base (insert y (B₁ \ {x})):=
+/-- We can exchange in both directions at one -/
+theorem base.strong_exchange (hB₁ : M.base B₁) (hB₂ : M.base B₂) (hx : x ∈ B₁ \ B₂) :
+  ∃ y ∈ B₂ \ B₁, M.base (insert x (B₂ \ {y})) ∧ M.base (insert y (B₁ \ {x})) :=
 begin
   by_contra, 
-  simp_rw [not_exists] at h, 
-  obtain ⟨C, ⟨hCB₂,hC⟩, hCunique⟩ :=   
-    hB₂.indep.unique_circuit_of_insert x (hB₂.insert_dep hx.2), 
+  simp_rw [not_exists, not_and] at h, 
   
+  obtain ⟨C, ⟨hCB₂,hC⟩, hCunique⟩ :=   
+  hB₂.indep.unique_circuit_of_insert x (hB₂.insert_dep hx.2), 
+  
+  have hCss := diff_singleton_subset_iff.mpr hCB₂, 
+
   simp only [exists_unique_iff_exists, exists_prop, and_imp] at hCunique, 
-  have hC_exchange : ∀ y ∈ C, y ≠ x →  M.base (insert x (B₂ \ {y})), 
-  { intros y hyC hyx, 
-    have hy₂ : y ∈ B₂, 
-      from mem_of_mem_insert_of_ne (hCB₂ hyC) hyx, 
-    rw [base_iff_indep_card, ncard_exchange hx.2 hy₂, hB₂.card, eq_self_iff_true, and_true],
+  have hC_exchange : ∀ y ∈ C \ {x}, M.base (insert x (B₂ \ {y})), 
+  { rintros y ⟨hyC, hyx⟩, 
+    
+    rw [base_iff_indep_card, ncard_exchange hx.2 (hCss ⟨hyC,hyx⟩), hB₂.card, eq_self_iff_true, 
+      and_true],
     by_contra hdep, 
     rw [dep_iff_supset_circuit] at hdep, 
     obtain ⟨C', hC'ss, hC'⟩ := hdep, 
@@ -34,41 +38,168 @@ begin
     subst this, 
     simpa using hC'ss hyC},
   
-  -- have hr : B₂ ⊆   
+  have hcl : ∀ y ∈ B₂ \ M.cl (B₁ \ {x}), M.base (insert y (B₁ \ {x})), 
+  { rintro y ⟨hy₂, hy₁⟩, 
+    obtain rfl | hyx := em (y = x), 
+    { rwa [insert_diff_singleton, insert_eq_self.mpr hx.1]},
+    have hyB₁ : y ∉ B₁, from 
+      λ hyB₁, hy₁ (M.subset_cl (B₁ \ {x}) (mem_diff_singleton.mpr ⟨hyB₁, hyx⟩)), 
+    simp_rw [base_iff_indep_card, indep_iff_r_eq_card, ncard_exchange hyB₁ hx.1, 
+      hB₁.card, eq_self_iff_true, and_true, ←hB₁.card, not_mem_cl.mp hy₁, 
+      (hB₁.indep.diff {x}).r, ncard_diff_singleton_add_one hx.1]},
 
-  -- have hr : M.r B₂ ≤ M.r (B₁ \ {x}), 
-  -- { refine (M.r_mono (subset_union_right (B₁ \ {x}) B₂)).trans_eq 
-  --     (r_union_eq_of_r_all_insert_le (λ y hy₂, _)),
-  --   have hyx : y ≠ x, { rintro rfl, exact hx.2 hy₂}, 
-  --   obtain hy₁ | hy₁ := em (y ∈ B₁), 
-  --   { rw [insert_eq_of_mem], rw mem_diff_singleton, exact ⟨hy₁, hyx⟩},
-  --   have hB := h _ ⟨hy₂,hy₁⟩, 
-  --   rw [base_iff_indep_card_eq_r, ncard_exchange hy₁ hx.1, hB₁.card, eq_self_iff_true, and_true, 
-  --     ←r_lt_card_iff_dep, nat.lt_iff_add_one_le] at hB,
-  --   apply @nat.le_of_add_le_add_right 1, 
-  --   convert hB, 
-  --   rw [(hB₁.indep.subset (diff_subset _ _)).r, eq_comm], 
-  --   refine ncard_insert_of_not_mem (by simpa)},
-  -- rw [(hB₁.indep.subset (diff_subset _ _)).r, hB₂.indep.r, hB₂.card_eq_card_of_base hB₁] at hr, 
-  -- exact (ncard_diff_singleton_lt_of_mem hx.1).not_le hr, 
-  -- The above is just a proof of the regular exchange axiom. Embarrassing! 
+  have hss : C \ {x} ⊆ M.cl (B₁ \ {x}), 
+  from λ y hy, by_contra (λ hy', h _ ⟨hCss hy, λ hy₁, hy' (M.subset_cl _ ⟨hy₁,hy.2⟩)⟩ 
+      (hC_exchange y hy) (hcl _ ⟨hCss hy,hy'⟩)), 
+    
+  have hx' := (hC.1.subset_cl_diff_singleton _).trans (cl_subset_cl_of_subset_cl hss) hC.2, 
+  rw [mem_cl, insert_diff_singleton, insert_eq_of_mem hx.1, hB₁.indep.r, (hB₁.indep.diff _).r, 
+    ←ncard_diff_singleton_add_one hx.1] at hx', 
+  simpa only [nat.succ_ne_self] using hx', 
 end     
 
+lemma base.rev_exchange (hB₁ : M.base B₁) (hB₂ : M.base B₂) (hx : x ∈ B₁ \ B₂) :
+  ∃ y ∈ B₂ \ B₁, M.base (insert x (B₂ \ {y})) :=
+(hB₁.strong_exchange hB₂ hx).imp (by {rintro y ⟨hy,h,-⟩, use [hy,h]})
 
--- def dual (M : matroid E) : matroid E := 
--- { base := λ B, M.base Bᶜ,
---   exists_base' := exists.elim M.exists_base (λ B hb, ⟨Bᶜ, by rwa compl_compl⟩),
---   base_exchange' := 
---   begin
---     rintro B₁ B₂ hB₁ hB₂ x ⟨hx₁,hx₂⟩, 
---     rw [←mem_compl_iff] at hx₂, 
---     rw [←not_mem_compl_iff] at hx₁, 
---     -- rw mem_compl
---     obtain ⟨y,hy,hB⟩ := hB₂.rev_exchange hB₁ ⟨hx₂, hx₁⟩, 
---     -- obtain ⟨y,⟨hy₁,hy₂⟩,hB⟩ := hB₁.rev_exchange hB₂ ⟨hx₂, hx₁⟩,
---     -- rw [mem_compl_iff] at hy₁ hy₂, 
---     rw [diff_eq_compl_inter, compl_compl] at hy,
---     refine ⟨y,hy, _⟩, 
---   end }
+section dual 
+
+/-- The dual of a matroid. Its bases are the complements of bases -/
+def dual (M : matroid E) : matroid E := 
+{ base := λ B, M.base Bᶜ,
+  exists_base' := exists.elim M.exists_base (λ B hb, ⟨Bᶜ, by rwa compl_compl⟩),
+  base_exchange' := 
+  begin
+    rintro B₁ B₂ hB₁ hB₂ x ⟨hx₁,hx₂⟩, 
+    rw [←mem_compl_iff] at hx₂, 
+    rw [←not_mem_compl_iff] at hx₁, 
+    obtain ⟨y,hy,hB⟩ := hB₂.rev_exchange hB₁ ⟨hx₂, hx₁⟩, 
+    rw [diff_eq_compl_inter, compl_compl] at hy,
+    refine ⟨y,hy, _⟩, 
+    rwa [←union_singleton, compl_union, diff_eq_compl_inter, compl_inter, compl_compl, 
+      singleton_union, inter_comm, ←diff_eq_compl_inter, ←insert_diff_singleton_comm],
+    rintro rfl, 
+    exact hx₁ hy.2, 
+  end }
+
+@[simp] lemma dual_base_iff : 
+  M.dual.base B ↔ M.base Bᶜ :=
+iff.rfl 
+
+@[simp] lemma dual_dual (M : matroid E): 
+  M.dual.dual = M :=
+by {ext, simp}
+
+lemma dual_inj (h : M₁.dual = M₂.dual) : 
+  M₁ = M₂ := 
+by {ext B, rw [←compl_compl B, ←dual_base_iff, h, dual_base_iff]}
+
+@[simp] lemma dual_inj_iff : 
+  M₁.dual = M₂.dual ↔ M₁ = M₂ := 
+⟨dual_inj, congr_arg _⟩   
+
+end dual
+
+lemma dual_indep_iff :
+  M.dual.indep X ↔ ∃ B, M.base B ∧ disjoint B X :=
+begin
+  simp_rw [indep_iff_subset_base, dual_base_iff], 
+  split, 
+  { rintro ⟨B, hB, hXB⟩, 
+    exact ⟨_,hB,by rwa [←subset_compl_iff_disjoint_left, compl_compl]⟩},
+  rintro ⟨B,hB,hBX⟩, 
+  exact ⟨Bᶜ,by rwa compl_compl,subset_compl_iff_disjoint_left.mpr hBX⟩,
+end 
+
+lemma dual_indep_iff_r : 
+  M.dual.indep X ↔ M.r Xᶜ = M.rk := 
+begin
+  rw [dual_indep_iff], 
+  split,
+  { rintros ⟨B,hB,hBX⟩, 
+    refine le_antisymm (M.r_le_rk _) _, 
+    rw ←subset_compl_iff_disjoint_right at hBX, 
+    rw [←hB.r],
+    exact M.r_mono hBX},
+  intro hr, 
+  obtain ⟨B, hB⟩ := M.exists_basis Xᶜ, 
+  refine ⟨B, hB.indep.base_of_rk_le_card _, subset_compl_iff_disjoint_right.mp hB.subset⟩,  
+  rw [←hB.indep.r, hB.r, hr], 
+end  
+
+lemma loop.dual_coloop (he : M.loop e) :
+  M.dual.coloop e :=
+begin
+  intros B hB, 
+  rw dual_base_iff at hB, 
+  simpa using he.not_mem_indep hB.indep, 
+end 
+
+lemma coloop.dual_loop (he : M.coloop e) :
+  M.dual.loop e :=
+begin
+  rw [loop_def, circuit_def, dual_indep_iff],
+  simp only [ssubset_singleton_iff, disjoint_singleton_right, not_exists, not_and, not_not_mem, 
+    forall_eq], 
+  exact ⟨he, empty_indep _⟩, 
+end 
+
+@[simp] lemma dual_coloop_if_loop :
+  M.dual.coloop e ↔ M.loop e :=
+⟨λ h, by {rw ← dual_dual M, exact h.dual_loop}, loop.dual_coloop⟩ 
+
+@[simp] lemma dual_loop_iff_coloop :
+  M.dual.loop e ↔ M.coloop e :=
+⟨λ h, by {rw ←dual_dual M, exact h.dual_coloop}, coloop.dual_loop⟩ 
+
+lemma dual_r_add_rk_eq (M : matroid E) (X : set E) : 
+  M.dual.r X + M.rk = ncard X + M.r Xᶜ  :=
+begin
+  set r₀ : (set E) → ℤ := λ X, nat.card E - M.nullity Xᶜ with hr₀, 
+  have hr₀_nonneg : ∀ X, 0 ≤ r₀ X, 
+  { sorry},
+  set r' := int.to_nat ∘ r₀ with hr', 
+  
+  have hr'_mono : ∀ X Y, X ⊆ Y → r' X ≤ r' Y,     
+  { sorry}, 
+  have hr'_le_card : ∀ X, r' X ≤ X.ncard,   
+  {sorry}, 
+  have hr'_submod : ∀ X Y, r' (X ∩ Y) + r' (X ∪ Y) ≤ r' X + r' Y, 
+  {sorry}, 
+
+  set M' := matroid_of_r r' hr'_le_card hr'_mono hr'_submod with hM',
+
+  have hM'M : M' = M.dual,
+  { ext B, 
+    
+    rw [hM', base_iff_indep_card_eq_r, indep_iff_r_eq_card, rk_def, matroid_of_r_apply, 
+      dual_base_iff, hr'], 
+    dsimp, 
+    rw [coe_nullity], 
+    
+    refine ⟨λ h, _,λ h, _⟩, 
+
+
+      
+       }, 
+
+  -- rw (@eq_r_iff _ _ M.dual X (X.ncard + M.r Xᶜ - M.rk)).mpr,
+  -- { refine nat.sub_add_cancel _, sorry },
+  -- obtain ⟨I, hI, hss, hmax⟩ := M.dual.exists_basis X,     
+  -- refine ⟨I, ⟨hI,hss,hmax⟩, _⟩, 
+  -- simp_rw [dual_indep_iff] at hI hmax, 
+  -- obtain ⟨B, hB, hBI⟩ := hI, 
+
+  
+  -- simp_rw [←add_left_inj (M.rk)] at this,  
+  -- zify, 
+  -- rw [eq_comm, add_comm, ←sub_eq_iff_eq_add, eq_comm],
+end 
+
+section rank
+
+
+
+end rank 
 
 end matroid 
